\documentclass{jn-pset}
%   \documentclass[solutions]{jn-pset}

\usepackage{ifthen}
\newboolean{versionwithsolutions}
% Uncomment to insert text that should only be there in version WITH solutions
\setboolean{versionwithsolutions}{true}
% Uncomment to insert text that should only be there in version WITHOUT solutions
\setboolean{versionwithsolutions}{false}


%%%%
%%%% QUICK INSTRUCTIONS FOR FORMATTING OF PROBLEMS
%%%%
%    
% Code a problem by
%    \begin{problem}
%    \end{problem}
%
% Code a subproblem inside a problem by (note the percent signs!)
%    \begin{subproblem}%
%        \label{problem:labelhere}%
%        Text here
%    \end{subproblem}
%
% Get a small vertical space by issuing the command
%    \smallskip
%
% To give a hint to a problem (after having completed the problem statement),
% use the following LaTeX code for formatting consistency:
%
%    \smallskip
%    \noindent
%    \emph{Hint:}
%    Consider the following super-useful hint for this particular problem...
%

% PROBLEM-SET-SPECIFIC MACROS (UPDATE FOR EACH PROBLEM SET)

\newcommand{\psetno}{2}
\newcommand{\duedate}{Wednesday February 25 at 12:59 CET}

\newcommand{\thresholdforpass}{$120$~points\xspace}

\input{course-macros.tex}

% For getting watermark "DRAFT" across all pages (for instance, 
% when posting preliminary version of problem set)
\usepackage{draftwatermark}
% \SetWatermarkFontSize{20 cm}
\SetWatermarkScale{5}

% For METAPOST logo as \hologo{METAPOST}
%   \usepackage{hologo}

% For TikZ
%   \input{Figures/tikz-packages.tex}

%%%
%%% TITLE
%%%

\author{\courseinstructor}
\course{\coursenamelong{}}
\semester{\courseperiod}
\title{\coursenameshort: Problem Set \psetno}

\begin{document}

\maketitle

\input{IDMA_Pset_GeneralInstructions}


%%%
%%% IDMA 2026 EXAM: PROBLEM 3
%%% Mathematical induction problem
%%%
\begin{problem}
  (60 p)
  Provide formal proofs of the following claims
  using proof techniques that we have learned during the course.


  \begin{subproblem}%
    \ifthenelse{\boolean{versionwithsolutions}}
    {(30 p)}
    {\ignorespaces}
    Define
    $a_1 = 1$
    and
    $a_n = 2 a_{n-1} + 1$
    for
    $n \geq 2$.
    Prove that for all positive integers
    $n \in \Nplus$
    it holds that 
    $a_n = 2^n - 1$.
  \end{subproblem}

\begin{solution}
We prove this equality by induction over~$n$.

\begin{description}
\item[\emph{Base case ($n=1$):}]
  We have
  $a_1 = 1 = 2^1 - 1$
  by definition.

\item[\emph{Induction step:}]
  Assume that the equality holds for $n-1$ and consider $n$.
  We have
  \begin{align*}
    a_n &= 2 a_{n-1} + 1
    \\                           
    &= 2 \cdot (2 ^{n-1} - 1) + 1
    &&[\text{by the induction hypothesis}]
    \\
    &= 2 ^{n} - 2 + 1    
    \\
    &= 2 ^{n} - 1
  \end{align*}
  which is the desired equality.
\end{description}
The claim now follows by the induction principle.  
\end{solution}


\begin{subproblem}%
  \ifthenelse{\boolean{versionwithsolutions}}
  {(30 p)}
  {\ignorespaces}
  Prove that for all non-negative integers
  $n \in \N$
  it holds that
  $
  3 \mid 4^n + 5 
  $.
\end{subproblem}

\begin{solution}
%     This is very similar to a problem we did in class, 
%     and we will solve this one in the same way by arguing by
  We prove this by 
  induction over~$n$.
  \begin{description}
  \item[\emph{Base case ($n=0$):}]
    For $n=0$ we have that
    $
    4^0 + 5 
    =
    6
    $
    is divisible by~$3$.
    
  \item[\emph{Induction step:}]
    Suppose that
    $
    3 \mid 4^n + 5
    $,
    which is the same  as saying that
    $
    4^n + 5 = 3 \cdot M
    $
    for some integer~$M$.
    Fixing this $M$, and
    working on the expression \mbox{for $n+1$}, we get
    \begin{align*}
      4^{n+1} + 5
      &= 
        3 \cdot 4^{n}
        + 
        4^{n} + 5
      &&[\text{since $4^{n+1} = (3 + 1) \cdot 4^n$}]
      \\
      &= 
        3 \cdot 4^{n}
        + 
        3 \cdot M
      &&[\text{by the induction hypothesis}]
      \\
      &=
        3 \cdot ( 4^{n} + M )
    \end{align*}
    which shows that this expression is divisible by~$3$.
  \end{description}
  The claim follows by the induction principle.
\end{solution}


\end{problem}

%%%
%%% IDMA EXAM 2026: PROBLEM 5
%%% PROPOSITIONAL LOGIC
%%%

\begin{problem}%
  \label{problem:logic}%
  (60 p)  
  For each of the propositional logic formulas below,
  determine whether it is a tautology or not.
  If the formula is not a tautology, show how to
  add a single connective to make it into a tautology.
  Please make sure to justify your answers
  (e.g., by presenting truth tables, or by using rules for rewriting logic formulas
  that we have learned in class).

%%% TAUTOLOGY  
  \begin{subproblem}%
    \label{problem:formula-1}%
    \ifthenelse{\boolean{versionwithsolutions}}
    {(30 p)}
    {\ignorespaces}
    $
    \lnot \bigl(
    ( p \limpl q) \lor r
    \bigr)
    \limpl
    \bigl(
    (\lnot q \land \lnot r) \land p
    \bigr)
    $
  \end{subproblem}

\begin{solution}
  This formula is a tautology, i.e., it is always true.
  To see this, note first that we know that
  \begin{equation}
    \label{eq:impl}
    p \limpl q
    \ \equiv \
    \lnot p \lor q
  \end{equation}
  since the only way the implication
  $p \limpl q$
  can be false is that $p$ is true and $q$ is false,
  and this is one of the basic equivalences we have learned in the course.
  Furthermore, from De Morgan's laws it is easy to derive that
  \begin{equation}
    \label{eq:de-morgan}
    \lnot ( a \lor b \lor c)
    \ \equiv \
    \lnot a \land \lnot b \land \lnot c
  \end{equation}
  (i.e., the only way a disjunction can be false is that all its
  disjuncts are false).
  
  By combining
  \eqref{eq:impl}
  and~\eqref{eq:de-morgan},
  and using that conjunction is commutative, we see that the premise
  $
  \lnot \bigl(
  ( p \limpl q) \lor r
  \bigr)
  $
  is in fact equivalent to the conclusion
  $
  (\lnot q \land \lnot r) \land p
  $,
  and so the implication
  in Problem~\ref{problem:formula-1}
  will always evaluate to true.
\end{solution}

  \begin{subproblem}
    \ifthenelse{\boolean{versionwithsolutions}}
    {(30 p)}
    {\ignorespaces}
    $
    \bigl(
    (p \land q) \limpl r
    \bigr)
    \lequiv
    \bigl(
    (q \lor r) \lor \lnot p
%%% This should be    
%       (\lnot q \lor r) \lor \lnot p
    \bigr)
    $    
  \end{subproblem}

\begin{solution}
  This is not a tautology.
  If we set $p$ and~$q$ to true
  but $r$ to false, we get that
  $
  (p \land q) \limpl r
  $
  evaluates to  false but
  $
  (q \lor r) \lor \lnot p
%%% This should be    
%       (\lnot q \lor r) \lor \lnot p
  $
  evaluates to true, and so the whole formula is false.

  If we change $q$ on the right-hand side to $\lnot q$,
  we obtain the formula
  \begin{equation}
    \label{eq:patched}
    \bigl(
    (p \land q) \limpl r
    \bigr)
    \lequiv
    \bigl(
    (\lnot q \lor r) \lor \lnot p
    \bigr)
    \ ,
  \end{equation}    
  which is a tautology. To see this, we can rewrite the left-hand side
  of~\eqref{eq:patched}
  as
  \begin{subequations}
  \begin{align}
    (p \land q) \limpl r
    \ &\equiv \
        \lnot (p \land q) \lor r
    \\
    \ &\equiv \
        (\lnot p \lor \lnot q) \lor r
    \\
    \ &\equiv \
        (\lnot q \lor r) \lor \lnot p
  \end{align}
  \end{subequations}
  by using
  the property~\eqref{eq:impl} of implication,
  De Morgan's laws,
  and commutativity of disjunction.
  This show that the left-hand and right-hand sides of
  of the formula~\eqref{eq:patched} are equivalent,
  and so the formula will always evaluate to true.
\end{solution}

\end{problem}


%%%
%%% DMFS 2023 PROBLEM SET 5: IDMA 2026 EXAM: PROBLEM 3
%%% Buggy induction proofs
%%%

\begin{problem} (60 p)
  When constructing this problem set, Jakob ran into some very unfortunate problems.
  When he wanted to add a couple of more examples illustrating
  the power of inductive proofs, the proofs
  turned out to be a little bit too powerful.
  Specifically, Jakob was able to use mathematical induction to
  show
  \begin{enumerate}
  \item
    that all swans have the same colour (presumably white, so that there
    are no black swans after all), and
    
  \item
    that all positive integers are in fact equal.
  \end{enumerate}
  %
  Both of these claims are fairly disturbing from a mathematical point
  of view.
  Please help Jakob by pointing out clearly what goes wrong in his
  induction proofs below.

  \begin{subproblem}
    \textbf{Theorem.} All swans have the same colour.

    \smallskip
    \noindent
    \emph{Proof.} We prove by induction over~$n$
    that any set of~$n$ swans have the same colour.
    
    For the base case, if we have a set of $n=1$ swan, then this swan
    vacuously has the same colour as itself.

    For the induction step, assume as our induction hypothesis  that
    all sets of $n$~swans have the same colour, and consider a set of
    $n+1$~swans. Fix some swan~$S_1$ in this set. If we remove~$S_1$,
    then we have $n$~swans left, and by the induction hypothesis they
    all have the same colour. Let~$C$ be this colour.

    Now consider another swan~$S_2$ in the set. If we remove~$S_2$
    from our set of $n+1$~swans instead of $S_1$, then we again have
    $n$~swans left, and they all have the same colour by the induction
    hypothesis. Since $S_1$ is one of the swans in this set, it must
    have the same colour~$C$ as all the others. Hence, all $n+1$~swans
    have the same colour.

    It follows by the principle of mathematical induction that any set
    of $n$~swans must always have the same colour.    
  \end{subproblem}

\begin{solution}
  The base case is correct.
  
  The induction step is also correct for all $n \geq 3$.
  It is true that if I have a set of $n \geq 3$~objects with the property
  that any  subset of $n-1$ objects must all have the same colour,
  then the only way this can happen is that all $n$~objects have the
  same colour. 

  
  However, for $n=2$ there is a gap in the argument, and this is why
  we can ``prove'' a false theorem. If we remove swan~$S_2$ from the
  set, then there is only swan~$S_1$ left. This swan~$S_1$ could have a
  different colour, contrary to what the induction step argument
  claims.

  
  
\end{solution}
  
  \begin{subproblem}
    \textbf{Theorem.} All positive integers are equal.
    
    \smallskip
    \noindent
    \emph{Proof.} By induction over~$n$.
    
    For the base case, the positive integer~$1$ is equal to itself.

    For the induction step, assume as our induction hypothesis that
    $n - 1 = n$.
    Adding~$1$ to both sides of this equality, we derive that
    $n = n + 1$.

    It follows from this by the principle of mathematical induction
    that for all integers~$n$ the equality $n = n + 1$ holds. But then
    by transitivity we obtain that all integers are equal, and the
    claim in the theorem statement has thus been established.    
  \end{subproblem}
  
\begin{solution}
  The induction step in this proof is just fine, but the base case is
  wrong.

  Since the induction hypothesis is that
  $n - 1 = n$,
  for the base case we would need to prove that
  $0=1$
  or
  $1=2$
  or something.
  But in the base case in the ``proof'' above, we are not
  proving a base case of the form $n-1=n$, but rather $n=n$.
  This is of course true, but this does not match what we need when we
  want to use the base case as induction hypothesis for our first
  induction step.
\end{solution}
  
  
\end{problem}



\end{document}


